proof/old_system/_.v
@@ -8,5 +8,8 @@ Require Import uni.decl_worklist.prop_equiv.
 Require Import uni.algo_worklist.transfer.
 Require Import uni.algo_worklist.def_extra.
 
+Require Import uni.algo_worklist.prop_soundness.
+Require Import uni.algo_worklist.prop_completness.
+Require Import uni.algo_worklist.prop_decidability.
 
 Print Assumptions d_chk_inf_subsumption.
