proof/old_system/uni/def_extra.v
@@ -4,21 +4,21 @@ Require Import List.
 Require Import uni.def_ott.
 
 
-Fixpoint ftvar_in_aworklist' (aW_5:aworklist) : vars :=
-  match aW_5 with
+Fixpoint ftvar_in_aworklist' (Γ_5:aworklist) : vars :=
+  match Γ_5 with
   | aworklist_empty => empty
-  | (aworklist_consvar aW x ab) => (ftvar_in_aworklist' aW) \u (ftvar_in_abind ab)
-  | (aworklist_constvar aW X ab) => (ftvar_in_aworklist' aW) \u (ftvar_in_abind ab) \u (singleton X)
-  | (aworklist_conswork aW w) => (ftvar_in_aworklist' aW) \u (ftvar_in_work w)
+  | (aworklist_consvar Γ x ab) => (ftvar_in_aworklist' Γ) \u (ftvar_in_abind ab)
+  | (aworklist_constvar Γ X ab) => (ftvar_in_aworklist' Γ) \u (ftvar_in_abind ab) \u (singleton X)
+  | (aworklist_conswork Γ w) => (ftvar_in_aworklist' Γ) \u (ftvar_in_work w)
 end.
 
 
-Fixpoint fvar_in_aworklist' (aW_5:aworklist) : vars :=
-  match aW_5 with
+Fixpoint fvar_in_aworklist' (Γ_5:aworklist) : vars :=
+  match Γ_5 with
   | aworklist_empty => {}
-  | (aworklist_consvar aW x ab) => (fvar_in_aworklist' aW) \u (singleton x) (* no var in abind *)
-  | (aworklist_constvar aW X ab) => (fvar_in_aworklist' aW) (* no var in abind *)
-  | (aworklist_conswork aW w) => (fvar_in_aworklist' aW) \u (fvar_in_work w)
+  | (aworklist_consvar Γ x ab) => (fvar_in_aworklist' Γ) \u (singleton x) (* no var in abind *)
+  | (aworklist_constvar Γ X ab) => (fvar_in_aworklist' Γ) (* no var in abind *)
+  | (aworklist_conswork Γ w) => (fvar_in_aworklist' Γ) \u (fvar_in_work w)
 end.
   
 
